Refactored Proof.v to reason about proof stages

theories/Proof.v
@@ -19,7 +19,7 @@ Inductive InferenceRule :=
   .
 
 Inductive Step := 
-| inference (fact : Deduction.Inference) (hint : list N) (rule : InferenceRule)
+  | inference (fact : Deduction.Inference) (hint : list N) (rule : InferenceRule)
   | nogood (fact : Deduction.Inference) (chain : list N).
 
 Definition step_fact (step : Step) :=
@@ -28,7 +28,35 @@ Definition step_fact (step : Step) :=
   | nogood fact _ => fact
   end.
 
-Definition CPProof := (list (N * Step))%type.
+Record HydratedInference := {
+  hinf_index : N ;
+  hinf_fact : Inference ;
+  hinf_hint : list Constraint ;
+  hinf_rule : InferenceRule
+}.
+
+Record HydratedProofStage := {
+  hs_inferences : list HydratedInference ;
+  hs_chain : list Inference ;
+  hs_conclusion : Inference ;
+  hs_conclusion_index : N
+}.
+
+Record IndexedInference := {
+  iinf_index : N ;
+  iinf_fact : Inference ;
+  iinf_hint : list N ;
+  iinf_rule : InferenceRule
+}.
+
+Record ProofStage := {
+  s_inferences : list IndexedInference ;
+  s_chain : list N ;
+  s_conclusion : Inference ;
+  s_conclusion_index : N
+}.
+
+Definition CPProof := (list ProofStage)%type.
 
 Definition validate_inference (fact : Deduction.Inference) (hint : list Constraint) (rule : InferenceRule) :=
   match rule with
@@ -81,159 +109,142 @@ Definition validate_nogood (fact : Inference) (chain : list Inference) :=
   end.
 
 
-Record ProofStage := {
-  s_inferences : list (N * Inference * (list Constraint) * InferenceRule) ;
-  s_conclusion : Inference * list Inference
-}.
 
-Definition validate_inference_within_stage (step : N * Inference * (list Constraint) * InferenceRule) : bool :=
-  match step with
-  | (_, fact, hint, rule) => validate_inference fact hint rule
-  end.
+Definition validate_inference_within_stage (step : HydratedInference) :=
+  validate_inference step.(hinf_fact) step.(hinf_hint) step.(hinf_rule).
 
 
-Definition validate_nogood_within_stage (step : (Inference * list Inference)) : bool :=
-  match step with
-  | (fact, chain) => validate_nogood fact chain
-  end.
-
-Definition validate_proof_stage (stage : ProofStage) :=
+Definition validate_proof_stage (stage : HydratedProofStage) :=
   (* Validate every inference independently *)
   let inferences_ok := forallb 
     validate_inference_within_stage
-    stage.(s_inferences)
+    stage.(hs_inferences)
   in
   (* Check that the conclusion is a valid deduction *)
-  let conclusion_ok := validate_nogood_within_stage stage.(s_conclusion) in
+  let conclusion_ok := validate_nogood stage.(hs_conclusion) stage.(hs_chain) in
   andb inferences_ok conclusion_ok.
   
 
-Definition used_constraints (stage : ProofStage) :=
-  let hints :=
-    flat_map (fun x => match x with
-                       | (_, cs, _) => cs
-                       end) stage.(s_inferences)
+Definition used_constraints (stage : HydratedProofStage) :=
+  let hints := flat_map hinf_hint stage.(hs_inferences)
   in
-  let (_, raw_inferences) := stage.(s_conclusion)
-  in
-  let inferences := map fact_c raw_inferences
+  let inferences := map fact_c stage.(hs_chain)
   in
   hints ++ inferences.
 
 
-
 Lemma valid_proof_stage_implies_conclusion : forall
-  (stage : ProofStage) (sol : string -> Z) (conclusion : Inference) (chain : list Inference),
+  (stage : HydratedProofStage) (sol : string -> Z),
   Is_true (validate_proof_stage stage) ->
-  stage.(s_conclusion) = (conclusion, chain) ->
   (forall (c : Constraint),
     In c (used_constraints stage) -> satisfies_constraint c sol
   ) ->
-  inference_valid sol conclusion.
+  inference_valid sol (stage.(hs_conclusion)).
 Proof.
-  intros stage sol conclusion chain Hvalid Estage_conclusion Hcons_sat.
+  intros stage sol Hvalid Estage_conclusion Hcons_sat.
   unfold validate_proof_stage in Hvalid.
   apply andb_prop_elim in Hvalid.
-  unfold validate_inference_within_stage, validate_nogood_within_stage in Hvalid.
+  unfold validate_inference_within_stage in Hvalid.
   destruct Hvalid as [Hinf_valid Hnogood_valid].
-  rewrite Estage_conclusion in Hnogood_valid.
   unfold validate_nogood in Hnogood_valid.
-  destruct conclusion.(i_consequent) eqn:Econs in Hnogood_valid ;
+  destruct stage.(hs_conclusion).(i_consequent) eqn:Econs in Hnogood_valid ;
   try contradiction.
-  unfold inference_valid.
   rewrite Econs.
-  intros Hvalid_atoms.
   apply Is_true_eq_true in Hinf_valid.
   rewrite forallb_forall in Hinf_valid.
   apply check_deduct_correct with
     (assignment := sol)
-    (premises := i_premises conclusion)
-    (steps := chain).
-  - exact Hvalid_atoms.
+    (premises := stage.(hs_conclusion).(i_premises))
+    (steps := stage.(hs_chain)).
+  - exact Hcons_sat.
   - intros inf Hin_inf.
-    specialize (Hcons_sat (fact_c inf)).
-    simpl in Hcons_sat.
-    apply Hcons_sat.
+    specialize (Estage_conclusion (fact_c inf)).
+    simpl in Estage_conclusion.
+    apply Estage_conclusion.
     unfold used_constraints.
-    rewrite Estage_conclusion.
     apply in_or_app.
     right.
     apply in_map, Hin_inf.
   - apply Is_true_eq_true, Hnogood_valid.
 Qed.
 
-
-Fixpoint validate_stateful (csp : ConstraintProblem) (p : CPProof)
-  (stage_facts : list (N * Inference * list Constraint * InferenceRule)) :=
-  match p with 
-  | nil => true
-  (* The next fact is a nogood; the proof stage is over, send it to the stage validator
-     and, if it approves, proceed with the rest of the proof while forgetting the inferences *)
-  | (step_index, nogood fact index_chain) :: p' =>
-      (* Unpack the fact from the inferences available on the current stage *)
-      let stage_lookup :=
-        fun index => flat_map
-          (fun stage_fact : (N * Inference * list Constraint * InferenceRule) =>
-            match stage_fact with
-            | (stage_index, i, _, _) =>
-                if N.eqb stage_index index
-                then [i]
-                else []
-            end)
-          stage_facts
+Fixpoint hydrate_deduction_chain (csp : ConstraintProblem) (infs : list IndexedInference) (index_chain : list N) : list Inference :=
+  match index_chain with
+  | nil => nil
+  | index :: tail =>
+      let chain_tail := hydrate_deduction_chain csp infs tail
       in
-      (* Unpack the fact from the CSP or forward to the stage lookup *)
-      let fact_lookup := 
-        fun index => match ConstraintProblem.lookup csp index with
-                     | Some (fact_c i) => [i]
-                     | _ => stage_lookup index
-                     end
-      in
-      (* Unpack all facts from the index chain *)
-      let chain := flat_map fact_lookup index_chain
-      in
-      (* Store all processed inferences and the newly found conclusion *)
-      let stage := {|
-        s_inferences := stage_facts ;
-        s_conclusion := (
-          fact,
-          chain
-        )
-      |}
-      in
-      (* Add the conclusion into the CSP *)
-      let csp' := ConstraintProblem.add
-        step_index
-        fact
-        csp
-      in
-      (* Keep checking if the stage is valid, declare failure otherwise *)
-      if validate_proof_stage stage
-      then validate_stateful csp' p' nil
-      else false
-  (* The next fact is an inference, append it with metadata and keep goind *)
-  | (step_index, inference fact hint_indices rule) :: p' =>
-      (* Extract the hint constraints *)
-      let lookup := fun index =>
+      let chain_head :=
         match ConstraintProblem.lookup csp index with
-        | Some c => [c]
-        | None => []
+        | Some (fact_c i) => [i]
+        | _ => map
+            (fun inf => inf.(iinf_fact))
+            (filter (fun inf => N.eqb (inf.(iinf_index)) index) infs)
         end
-      in
-      let hint := flat_map lookup hint_indices
-      in
-      (* Store the inference in memory and proceed further *)
-      validate_stateful csp p' ((step_index, fact, hint, rule) :: stage_facts)
+      in chain_head ++ chain_tail
   end.
 
-Definition validate (csp : ConstraintProblem) (p : CPProof) := validate_stateful csp p nil.
+
+Lemma hydrated_chain_lookup : forall
+  (csp : ConstraintProblem) (infs : list IndexedInference) (index_chain : list N)
+  (fact : Inference),
+  In fact (hydrate_deduction_chain csp infs index_chain) ->
+  (exists x, ConstraintProblem.lookup csp x = Some (fact_c fact)) \/
+  (exists inf, In inf infs /\ inf.(iinf_fact) = fact).
+Admitted.
+
+
+Definition hydrate_inference (csp : ConstraintProblem) (inf : IndexedInference) : HydratedInference :=
+  let hint := flat_map (
+    fun index =>
+    match ConstraintProblem.lookup csp index with
+    | Some c => [c]
+    | None => []
+    end
+  )
+  (inf.(iinf_hint))
+  in
+  {|
+    hinf_index := inf.(iinf_index) ;
+    hinf_fact := inf.(iinf_fact) ;
+    hinf_hint := hint ;
+    hinf_rule := inf.(iinf_rule)
+  |}.
+
+
+Definition hydrate (csp : ConstraintProblem) (stage : ProofStage) : HydratedProofStage :=
+  let inferences := map (hydrate_inference csp) stage.(s_inferences)
+  in
+  let chain := hydrate_deduction_chain csp stage.(s_inferences) stage.(s_chain)
+  in
+  {|
+    hs_inferences := inferences ;
+    hs_conclusion := stage.(s_conclusion) ;
+    hs_chain := chain ;
+    hs_conclusion_index := stage.(s_conclusion_index) ;
+  |}
+  .
+
+
+Fixpoint validate (csp : ConstraintProblem) (p : CPProof) :=
+  match p with
+  | nil => true
+  | stage :: p' =>
+      let csp' := ConstraintProblem.add
+        (stage.(s_conclusion_index))
+        (stage.(s_conclusion))
+        csp
+      in
+      if validate_proof_stage (hydrate csp stage)
+      then validate csp' p'
+      else false
+  end.
 
 
 Fixpoint conclusion (p : CPProof) := 
   match p with
   | [] => None
-  | [(_, nogood fact _)] => Some fact
-  | [(_, inference _ _ _)] => None
+  | [stage] => Some (stage.(s_conclusion))
   | _ :: p' => conclusion p'
   end.
 
@@ -244,258 +255,119 @@ Definition conclusion_holds (csp : ConstraintProblem) (fact : Deduction.Inferenc
     Deduction.inference_valid sol fact.
 
 
-Definition used_constraints_memory
-  (mem : list (N * Inference * list Constraint * InferenceRule)) :=
-  flat_map
-  (
-    fun x : N * Inference * list Constraint * InferenceRule =>
-    match x with
-    | (_, _, c, _) => c
-    end
-  )
-  mem.
-
-Lemma nogood_stateful_soundness : forall
-  (csp : ConstraintProblem) (p : CPProof) (fact : Deduction.Inference) chain index
-  (mem : list (N * Inference * list Constraint * InferenceRule)),
-  (forall (c : Constraint),
-    In c (used_constraints_memory mem) ->
-    exists c_index, lookup csp c_index = Some c
-  ) ->
-  Is_true (validate_stateful csp ((index, nogood fact chain) :: p) mem) ->
-  conclusion_holds csp fact.
+Theorem step_soundness : forall
+  (csp : ConstraintProblem) (p : CPProof) (stage : ProofStage),
+    Is_true (validate csp (stage :: p)) ->
+    conclusion_holds csp (stage.(s_conclusion)).
 Proof.
-  unfold conclusion_holds.
-  intros csp p fact chain index mem Hmem Hvalid sol Hsat.
+  intros csp p stage Hvalid.
   simpl in Hvalid.
-  remember (
-  flat_map
-  (fun index => match lookup csp index with
-                | Some (fact_c i) => [i]
-                | _ => flat_map
-                    (fun stage_fact : (N * Inference * list Constraint * InferenceRule) =>
-                    match stage_fact with
-                    | (stage_index, i, _, _) =>
-                        if N.eqb stage_index index
-                        then [i]
-                        else []
-                    end)
-                    mem
-                end)
-                chain
-  ) as full_chain.
-  remember {|
-    s_inferences := mem ;
-    s_conclusion := (fact, full_chain)
-  |} as stage.
-  destruct (validate_proof_stage stage) eqn:Evalid; try contradiction.
-  apply valid_proof_stage_implies_conclusion with (stage := stage) (chain := full_chain).
-  - rewrite Evalid.
+  (* Show that the proof checker on the hydrated stage returns true *)
+  remember (hydrate csp stage) as h_stage.
+  destruct (validate_proof_stage h_stage) eqn:Evalid ;
+  try contradiction.
+  clear Hvalid.
+  (* Destruct all parts of the stage definition *)
+  destruct stage as [inferences chain conclusion conclusion_index].
+  simpl.
+  rewrite Heqh_stage in Evalid.
+  unfold hydrate in Evalid.
+  simpl in Evalid.
+  (* Appeal to the proof stage checker soundness *)
+  unfold conclusion_holds.
+  intros sol Hsat.
+  assert (Hrewrite: conclusion = (hs_conclusion h_stage)). {
+    rewrite Heqh_stage.
     reflexivity.
-  - rewrite Heqstage.
+  }
+  rewrite Hrewrite.
+  clear Hrewrite.
+  apply valid_proof_stage_implies_conclusion.
+  - (* Rewrite into the proof checker validity *)
+    unfold hydrate in Heqh_stage.
+    simpl in Heqh_stage.
+    rewrite <- Heqh_stage in Evalid.
+    rewrite Evalid.
     reflexivity.
-  - intros c Hin_cons.
-    unfold used_constraints_memory.
-    rewrite Heqstage in Hin_cons.
+  - (* Show that any constraint used by the _hydrated_ stage is valid *)
+    intros c Hin_cons.
     unfold used_constraints in Hin_cons.
-    simpl in Hin_cons.
-    apply in_app_or in Hin_cons.
-    destruct Hin_cons as [Hin_mem | Hin_chain].
-    + specialize (Hmem c).
-      unfold used_constraints_memory in Hmem.
-      assert (Hmem':
-        In c
-        (flat_map
-        (fun x : N * Inference * list Constraint * InferenceRule =>
-        let (p, _) := x in let (p0, c) := p in let (_, _) := p0 in c) mem)
-      ). {
-        apply in_flat_map.
-        apply in_flat_map in Hin_mem.
-        destruct Hin_mem as [x [Hin_mem Hin_hint]].
-        destruct x as [x rule'].
-        destruct x as [x hint'].
-        destruct x as [index' fact'].
-        exists (index', fact', hint', rule').
-        split ; easy.
-      }
-      apply Hmem in Hmem'.
-      destruct Hmem'.
-      apply sat_csp_implies_sat_lookup with (csp := csp) (index := x) ; easy.
-    + apply in_map_iff in Hin_chain.
-      destruct Hin_chain as [fact' [Efact' Hin_fact']].
-      rewrite Heqfull_chain in Hin_fact'.
-      apply in_flat_map in Hin_fact'.
-      destruct Hin_fact' as [index' [Hin_chain Hlookup]].
-      remember (
-        flat_map
-          (fun stage_fact : N * Inference * list Constraint * InferenceRule
-           =>
-           let (p0, _) := stage_fact in
-           let (p1, _) := p0 in
-           let (stage_index, i) := p1 in
-           if (stage_index =? index')%N then [i] else []) mem
-      ) as mem_lookup eqn:Emem_lookup.
-      assert (Hlookup_sat: In fact' mem_lookup -> satisfies_constraint c sol). {
-        intros Hin_mem.
-        rewrite Emem_lookup in Hin_mem.
-        apply in_flat_map in Hin_mem.
-        destruct Hin_mem as [x [Hin_x Hin_fact']].
-        destruct x as [x rule''].
-        destruct x as [x hint''].
-        destruct x as [index'' fact''].
-        destruct (index'' =? index')%N ; simpl in Hin_fact' ; try contradiction.
-        destruct Hin_fact' as [Hin_fact' | F] ; try contradiction.
-        rewrite Heqstage in Evalid.
+    apply in_app_iff in Hin_cons.
+    destruct Hin_cons as [Hin_hint | Hin_chain].
+    + (* The constraint in question has been found in the hint.
+          Look up the constraint in the CSP and appeal to the CSP definition. *)
+      apply in_flat_map in Hin_hint.
+      destruct Hin_hint as [h_inf [Hin_inf Hin_hint]].
+      rewrite Heqh_stage in Hin_inf.
+      simpl in Hin_inf.
+      apply in_map_iff in Hin_inf.
+      destruct Hin_inf as [i_inf [Eh_inf Hin_inf]].
+      rewrite <- Eh_inf in Hin_hint.
+      simpl in Hin_hint.
+      apply in_flat_map in Hin_hint.
+      destruct Hin_hint as [index [Hin_hint Hin_c]].
+      destruct (lookup csp index) eqn:Elookup; try contradiction.
+      simpl in Hin_c.
+      destruct Hin_c as [Hin_c | F] ; try contradiction.
+      rewrite Hin_c in Elookup.
+      apply sat_csp_implies_sat_lookup with 
+        (csp := csp) (index := index) ; easy.
+    + (* The constraint in question has been found in the inference chain.
+         Use the lemma `hydrated_chain_lookup` *)
+      apply in_map_iff in Hin_chain.
+      destruct Hin_chain as [fact [Efact_c Hin_chain]].
+      rewrite Heqh_stage in Hin_chain.
+      simpl in Hin_chain.
+      apply hydrated_chain_lookup in Hin_chain.
+      destruct Hin_chain as [Hlookup|Hin_inferences].
+      * (* The fact was introduced from the CSP; appeal to the CSP definition. *)
+        destruct Hlookup as [index Elookup].
+        rewrite <- Efact_c.
+        apply sat_csp_implies_sat_lookup with
+          (csp := csp) (index := index) ; easy.
+      * (* The fact was introduced from the inference chain. Appeal to the 
+           correctness of the inference checker. *)
+        destruct Hin_inferences as [inf [Hin_inf Einf_fact]].
         unfold validate_proof_stage in Evalid.
-        apply andb_prop in Evalid.
-        destruct Evalid as [Evalid_inf Evalid_nogood].
-        simpl in Evalid_inf.
-        rewrite forallb_forall in Evalid_inf.
-        specialize Evalid_inf with (x := (index'', fact'', hint'', rule'')).
-        apply Evalid_inf in Hin_x as Evalid_inf'.
-        unfold validate_inference_within_stage in Evalid_inf'.
-        rewrite <- Efact', <- Hin_fact'.
+        apply Is_true_eq_left, andb_prop_elim in Evalid.
+        destruct Evalid as [Hvalid_inferences _].
+        apply Is_true_eq_true in Hvalid_inferences.
+        rewrite forallb_forall in Hvalid_inferences.
+        simpl in Hvalid_inferences.
+        unfold validate_inference_within_stage in Hvalid_inferences.
+        rewrite <- Efact_c.
         simpl.
-        apply validate_inference_soundness with (hint := hint'') (rule := rule'').
-        - intros.
-          specialize (Hmem c0).
-          cut (exists c_index : N, lookup csp c_index = Some c0).
-          + intros Hlookup_c0.
-            destruct Hlookup_c0.
-            apply sat_csp_implies_sat_lookup with (csp := csp) (index := x) ; easy.
-          + apply Hmem.
-            unfold used_constraints_memory.
-            apply in_flat_map.
-            exists (index'', fact'', hint'', rule'').
-            split ; easy.
-        - rewrite Evalid_inf'.
-          reflexivity.
-      }
-      destruct (lookup csp index') as [c'|] eqn:Elookup.
-      * destruct c' ; try apply Hlookup_sat, Hlookup.
-        simpl in Hlookup.
-        destruct Hlookup ; try contradiction.
-        rewrite H, Efact' in Elookup.
-        apply sat_csp_implies_sat_lookup with (csp := csp) (index := index').
-        -- exact Elookup.
-        -- exact Hsat.
-      * apply Hlookup_sat, Hlookup.
-Qed.
-
-Theorem stateful_soundness : forall
-  (csp : ConstraintProblem) (p : CPProof) (fact : Deduction.Inference)
-    (mem : list (N * Inference * list Constraint * InferenceRule)),
-    conclusion p = Some fact ->
-    (forall (c : Constraint),
-      In c (used_constraints_memory mem) ->
-      exists c_index, lookup csp c_index = Some c
-    ) ->
-    Is_true (validate_stateful csp p mem) ->
-    conclusion_holds csp fact.
-Proof.
-  intros csp p fact mem Econcl Hmem Hvalid.
-  generalize dependent mem.
-  generalize dependent csp.
-  induction p ; try discriminate.
-  (* Induction by proof length; base case p = nil is vacuously true. *)
-  intros csp mem Hmem Hvalid.
-  remember (a :: p) as p' eqn:Ep'.
-  destruct a.
-  destruct s.
-  + (* The upcoming step is an inference. Use inference soundness to
-       show that the memory invariant Hmem holds after adding this
-       inference with hint constraints. *)
-    remember (
-    flat_map (fun ix =>
-    match lookup csp ix with
-    | Some c => [c]
-    | None => []
-    end) hint) as full_hint eqn:Ehint.
-    remember ((n, fact0, full_hint, rule) :: mem) as mem'.
-    (* Apply the induction hypothesis with updated memory *)
-    apply IHp with (mem := mem').
-    - (* Conclusion in the new state is the same. *) 
-      simpl in Econcl.
-      rewrite Ep' in Econcl.
-      destruct p ; inversion Econcl.
-      destruct p.
-      destruct s ;
-      simpl in Econcl ;
-      rewrite Econcl ;
-      simpl ;
-      rewrite H0 ;
-      reflexivity.
-    - (* Memory invariant holds. *)
-      intros.
-      rewrite Heqmem' in H.
-      simpl in H.
-      apply in_app_or in H.
-      destruct H.
-      * (* Prove validity of hint constraints *)
-        rewrite Ehint in H.
-        apply in_flat_map in H.
-        destruct H.
-        destruct H.
-        destruct (lookup csp x) eqn:Elookup ; try contradiction.
-        simpl in H0.
-        destruct H0 ; try contradiction.
-        exists x.
-        rewrite Elookup, H0.
-        reflexivity.
-      * (* Prove validity of constraints inserted earlier *)
-        apply Hmem, H.
-    - (* Checker reports true on the proof suffix with updated memory *)
-      rewrite Ep' in Hvalid.
-      simpl in Hvalid.
-      rewrite <- Ehint, <- Heqmem' in Hvalid.
-      exact Hvalid.
-  + (* The upcoming step is a nogood. Use the special case lemma
-       to show that this fact is entailed by CSP, observe that 
-       the conclusion of the proof does not get invalidated by
-       adding an entailed constraint, and, if needed, apply the 
-       induction hypothesis. *)
-    assert (Hholds: conclusion_holds csp fact0). {
-      apply nogood_stateful_soundness with (p := p) (chain := chain) (index := n) (mem := mem).
-      + exact Hmem.
-      + rewrite <- Ep'.
-        exact Hvalid.
-    }
-    destruct p eqn:Ep.
-    - (* The proof suffix is a nogood and nothing else.
-         Use the special case above to close the goal. *)
-      rewrite Ep' in Econcl.
-      simpl in Econcl.
-      inversion Econcl.
-      rewrite H0 in Hholds.
-      exact Hholds.
-    - (* The upcoming step is a nogood, with more steps on the way.
-         Apply the induction hypothesis. *)
-      unfold conclusion_holds.
-      apply entailed_addition with (fact := fact0) (index := n) ;
-      try exact Hholds.
-      remember (add n fact0 csp) as csp'.
-      unfold conclusion_holds in IHp.
-      apply IHp with (mem := []) (csp := csp').
-      * (* Proof conclusion stays the same, as it is not empty. *)
-        rewrite Ep' in Econcl.
-        destruct p ; inversion Ep.
-        remember (p0 :: l) as q eqn:Eq.
-        simpl in Econcl.
-        destruct q ; inversion Eq.
-        rewrite <- Eq.
-        exact Econcl.
-      * (* The next run starts with an empty memory *)
-        intros.
-        contradiction.
-      * (* Checker reports true on the upcoming proof prefix
-           after mutating the CSP *)
-        rewrite Ep' in Hvalid.
-        remember (p0 :: l) as q.
-        simpl in Hvalid.
-        rewrite <- Heqcsp' in Hvalid.
-        destruct (validate_stateful csp' q []) ; try easy.
-        rewrite <- andb_lazy_alt, andb_false_r in Hvalid.
-        contradiction.
+        remember (hydrate_inference csp inf) as hinf.
+        apply validate_inference_soundness with
+          (hint := (hinf_hint hinf)) 
+          (rule := (hinf_rule hinf)).
+          -- (* Check that the hydrated hints are in the CSP *)
+             intros c' Hin_hint.
+             rewrite Heqhinf in Hin_hint.
+             simpl in Hin_hint.
+             apply in_flat_map in Hin_hint.
+             destruct Hin_hint as [index' [Hin_inf' Hin_c']].
+             destruct (lookup csp index') eqn:Elookup' ; try contradiction.
+             simpl in Hin_c'.
+             destruct Hin_c' as [Hin_c' | F] ; try contradiction.
+             rewrite Hin_c' in Elookup'.
+             apply sat_csp_implies_sat_lookup with (csp := csp) (index := index') ;
+             try easy.
+          -- (* Check that the inference checker returns true *)
+             assert (Hrewrite: fact = (hinf_fact hinf)). {
+               rewrite Heqhinf.
+               simpl.
+               rewrite Einf_fact.
+               reflexivity.
+             }
+             rewrite Hrewrite.
+             clear Hrewrite.
+             apply
+               Is_true_eq_left,
+               Hvalid_inferences with (x := hinf),
+               in_map_iff.
+             exists inf.
+             split ; easy.
 Qed.
 
 
@@ -505,12 +377,40 @@ Theorem soundness : forall
     Is_true (validate csp p) ->
     conclusion_holds csp fact.
 Proof.
-  intros.
-  apply stateful_soundness with (p := p) (mem := []).
-  - exact H.
-  - simpl.
-    intros.
-    contradiction.
-  - unfold validate in H0.
-    exact H0.
+  intros csp p fact Hconcl Hvalid.
+  generalize dependent csp.
+  (* Induction by proof length; base case p = nil is vacuously true. *)
+  induction p as [|stage] ; try discriminate.
+  intros csp Hvalid.
+  destruct p eqn:Ep.
+  (* The proof has a single stage; use stage checker soundness directly
+     after appropriately unpacking all variables *)
+  {
+    inversion Hconcl as [Hconcl'].
+    apply step_soundness with (p := nil).
+    exact Hvalid.
+  }
+  (* Use the induction hypothesis for the remainder of the proof and
+     the mutated CSP problem instance *)
+  assert (Hholds: conclusion_holds csp (stage.(s_conclusion))). {
+    apply step_soundness with (p := p0 :: l).
+    exact Hvalid.
+  }
+  unfold conclusion_holds.
+  apply entailed_addition with
+    (fact := stage.(s_conclusion))
+    (index := stage.(s_conclusion_index)) ;
+    try exact Hholds.
+  remember (add (stage.(s_conclusion_index)) (stage.(s_conclusion)) csp) as csp'.
+  unfold conclusion_holds in IHp.
+  apply IHp with (csp := csp').
+  + (* Proof conclusion stays the same, as it is not empty. *)
+    easy.
+  + (* Checker reports true on the upcoming proof prefix
+       after mutating the CSP *)
+    remember (p0 :: l) as q.
+    unfold validate in Hvalid.
+    rewrite <- Heqcsp' in Hvalid.
+    destruct (validate_proof_stage (hydrate csp stage)) ; try easy.
 Qed.
+
